examples/fac_master/tzwrap/fa2/multi_asset/FA2Types.v
@@ -12,6 +12,7 @@ Open Scope N.
 
 Section FA2Types.
 Context {BaseTypes: ChainBase}.
+Set Nonrecursive Elimination Schemes.
 
 Definition Ledger := FMap (Address * token_id) N.
 
@@ -19,20 +20,24 @@ Definition OperatorStorage := FMap (Address * (Address * token_id)) unit.
 
 Definition TokenTotalSupply := FMap token_id N.
 
-Record MultiTokenStorage :=  
-    mkMultiTokenStorage  {
+Record MultiTokenStorage :=   {
         ledger : Ledger ;
         operators : OperatorStorage ; 
         token_total_supply : TokenTotalSupply ;
         token_metadata : TokenMetaDataStorage
     }.
 
-Record MultiAssetStorage := 
-    mkMultiAssetStorage {
+Global Instance MultiTokenStorage_serializable : Serializable MultiTokenStorage :=
+Derive Serializable MultiTokenStorage_rect<Build_MultiTokenStorage>.
+
+Record MultiAssetStorage :=  {
         admin : TokenAdminStorage ; 
         assets : MultiTokenStorage ; 
         metadata : ContractMetadata
     }.
+
+Global Instance MultiAssetStorage_serializable : Serializable MultiAssetStorage :=
+Derive Serializable MultiAssetStorage_rect<Build_MultiAssetStorage>.
 
 Definition Return: Type := (MultiAssetStorage * (list ActionBody)).
 
