examples/fac_master/tzwrap/fa2/multi_asset/FA2_Multi_Asset.v
@@ -7,15 +7,24 @@ Require Import TokenAdmin.
 Require Import FA2_Multi_Token.
 Require Import Token_Manager.
 Require Import Monads.
+Require Import ZArith.
+Require Import Containers.
+Require Import String.
+Require Import List.
+Require Import Serializable.
 
 
 Section FA2_Multi_Asset.
 Context {BaseTypes : ChainBase}.
+Set Nonrecursive Elimination Schemes.
 
 Inductive MultiAssetParam :=
 | Assets (param : FA2EntryPoints)
 | Admin (param : MultiTokenAdmin)
 | Tokens (param : TokenManager).
+
+Global Instance MultiAssetParam_serializable : Serializable MultiAssetParam :=
+Derive Serializable MultiAssetParam_rect<Assets, Admin, Tokens>.
 
 Definition main (ctx : ContractCallContext) (param : MultiAssetParam) (s : MultiAssetStorage) : option Return :=
     match param with
@@ -31,5 +40,36 @@ Definition main (ctx : ContractCallContext) (param : MultiAssetParam) (s : Multi
         let new_s := s<| assets := fst tpl |> in
         Some (new_s, snd tpl)
     end.
+
+Definition fa2_receive (chain : Chain) (ctx : ContractCallContext) (state: MultiAssetStorage) (msg_opt : option MultiAssetParam) : option Return :=
+    do msg <- msg_opt ;
+    main ctx msg state.    
+
+Definition fa2_init (chain : Chain) (ctx: ContractCallContext) (setup: ((Address * Address) * ((list TokenMetadata) * N))) : option MultiAssetStorage :=
+    let (t1,t2) := setup in
+    let (admin, minter) := t1 in
+    let (tokens, meta_data_uri) := t2 in
+    let meta := FMap.update EmptyString (Some meta_data_uri) FMap.empty in
+    let token_metadata := fold_right (fun (token_metadata : TokenMetadata) (acc : TokenMetaDataStorage) => FMap.update token_metadata.(tm_token_id) (Some token_metadata) acc) FMap.empty tokens in
+    let supply := fold_right (fun (token_metadata : TokenMetadata) (acc : TokenTotalSupply) => FMap.update token_metadata.(tm_token_id) (Some 0) acc) FMap.empty tokens in
+    Some ({|
+        admin := {|
+            tas_admin := admin ;
+            tas_pending_admin := None ;
+            tas_paused := FMap.empty ;
+            tas_minter := minter
+        |} ;
+        assets := {|
+            ledger := FMap.empty ;
+            operators := FMap.empty ;
+            token_metadata := token_metadata ;
+            token_total_supply := supply
+        |} ;
+        metadata := meta
+    |}).
+
+(** The FA2 Contract **)
+Definition FA2_contract : Contract ((Address * Address) * ((list TokenMetadata) * N)) MultiAssetParam MultiAssetStorage :=
+    build_contract fa2_init fa2_receive.
 
 End FA2_Multi_Asset.
